OCaml Queue: proof of memory safety for [copy_aux] (wip).

examples/MList/MList.ml
@@ -19,6 +19,13 @@ let pop p =
   | Nil -> assert false
   | Cons (x,q) -> p := !q; x
 
+let rec copy p =
+  match !p with
+  | Nil -> ref Nil
+  | Cons (x, q) ->
+      let ll = copy q in
+      ref (Cons (x, ll))
+
 let rec rev_aux acc l =
   match !l with
   | Nil -> acc
@@ -33,7 +40,26 @@ let rev_main p =
 let rec cmp (eq: 'a -> 'a -> bool) l1 l2 =
   match !l1, !l2 with
   | Nil, Nil -> true
-  | Cons (_, _), Nil -> false
-  | Nil, Cons (_, _) -> false
+  | Cons (_, _), Nil | Nil, Cons (_, _) -> false
   | Cons (x1, xs1), Cons (x2, xs2) ->
       eq x1 x2 && cmp eq xs1 xs2
+
+let is_null p =
+  match !p with
+  | Nil -> true
+  | _ -> false
+
+let rec fold_mleft f acc p =
+  match !p with
+  | Nil -> acc
+  | Cons (x, q) -> fold_mleft f (f acc x) q
+
+let rec iter f p =
+  match !p with
+  | Nil -> ()
+  | Cons (x, q) -> f x; iter f q
+
+let test_iter (l: int mlist) =
+  let c = ref 0 in
+  iter (fun _ -> c := !c + 1) l;
+  !c
